day12-etc/Main.lean
@@ -2,5 +2,6 @@ import Day12Etc
 
 def main (args: List String) : IO Unit := do
   match args with
-  | "12_1"::xs => Day12.main xs
+  | "12_1"::xs => Day12.main false xs
+  | "12_2"::xs => Day12.main true xs
   | _ => IO.println "invalid args"
